extracted/ordered.ml
@@ -68,7 +68,7 @@ let node_to_graph (node : Lustre.node) : graph * (int, vertex) Hashtbl.t =
   in
   Stdlib.List.iter
     (fun (v, exp) ->
-      let vars = remove_dup @@ Lustre.var_of_exp exp in
+      let vars = remove_dup @@ LustreAst.var_of_exp exp in
       Stdlib.List.iter (fun u -> ignore @@ var_idx u) vars;
       g.(var_idx v) <- vars)
     node.n_body;
