theories/Languages/Lustre.v
@@ -1,89 +1,41 @@
 From Reactive Require Import Base.
 From Reactive.Datatypes Require Dict Stream.
+From Reactive.Languages Require LustreAst.
+
 
 From Coq Require Import Permutation String.
 
-Inductive type: Type :=
-  | TVoid
-  | TBool
-  | TInt.
+Module LustreAst := LustreAst.
 
-Definition binder := prod ident type.
-
-Inductive const: Type :=
-  | CVoid: const
-  | CBool: bool -> const
-  | CInt: nat -> const.
-
-(** A unary operator
-
-  An operator of type [unop tyin tyout] takes an argument of type [tyin] and
-  returns an expression of type [tyout].
-*)
-Inductive unop: Type :=
-  | Uop_not: unop
-  | Uop_neg: unop.
-
-(** A binary operator
-
-  An operator of type [binop ty1 ty2 tyout] takes two arguments of type [ty1]
-  and [ty2] returns an expression of type [tyout].
-*)
-Inductive binop: Type :=
-  (** Boolean binop *)
-  | Bop_and: binop
-  | Bop_or: binop
-  | Bop_xor: binop
- 
-  (** Arithmetic binop *)
-  | Bop_plus: binop
-  | Bop_minus: binop
-  | Bop_mult: binop
-  | Bop_div: binop
-  
-  (** Relational binop *)
-  | Bop_eq: binop
-  | Bop_le: binop
-  | Bop_lt: binop
-  | Bop_ge: binop
-  | Bop_gt: binop.
-
-Inductive exp: Type :=
-  | EConst: const -> exp
-  | EInput: binder -> exp
-  | EVar: binder -> exp
-  | EUnop: unop -> exp -> exp
-  | EBinop: binop -> exp -> exp -> exp
-  | EIfte: exp -> exp -> exp -> exp.
-
-Fixpoint has_einput (e: exp): bool :=
-  match e with
-    | EInput _ => true
-    | EConst _ | EVar _ => false
-    | EUnop _ e => has_einput e
-    | EBinop _ e1 e2 => has_einput e1 || has_einput e2
-    | EIfte e1 e2 e3 => has_einput e1 || has_einput e2 || has_einput e3
-  end.
-
-Definition equation := prod ident exp.
+Definition binder := LustreAst.binder.
 
 Record node := mk_node {
-  n_name: string;
+  node_ast :> LustreAst.node;
 
-  n_in: list binder;
-  n_out: binder;
-  n_locals: list binder;
-  n_body: list equation;
-
-  n_vars: list binder := n_in ++ n_out :: n_locals;
-  n_assigned_vars: list ident := map fst n_body;
+  n_vars: list binder := LustreAst.n_in node_ast ++ (LustreAst.n_out node_ast) :: (LustreAst.n_locals node_ast);
+  n_assigned_vars: list ident := map fst (LustreAst.n_body node_ast);
 
   n_assigned_vars_are_vars: incl n_assigned_vars (map fst n_vars);
-  n_assigned_out: In (fst n_out) n_assigned_vars;
-  n_out_is_not_an_input: ~ In n_out n_in;
-  n_inputs_equations: incl (List.map (fun b => (fst b, EInput b)) n_in) n_body;
-  n_no_einputs_in_other: Forall (fun '(name, exp) => ~ In name (map fst n_in) -> has_einput exp = false) n_body;
+  n_assigned_out: In (fst (LustreAst.n_out node_ast)) n_assigned_vars;
+  n_out_is_not_an_input: ~ In (LustreAst.n_out node_ast) (LustreAst.n_in node_ast);
+  n_inputs_equations: incl (List.map (fun b => (fst b, LustreAst.EInput b)) (LustreAst.n_in node_ast)) (LustreAst.n_body node_ast);
+  n_no_einputs_in_other: Forall (fun '(name, exp) => ~ In name (map fst (LustreAst.n_in node_ast)) -> LustreAst.has_einput exp = false) (LustreAst.n_body node_ast);
 }.
+
+
+
+Definition n_name (n:node) := LustreAst.n_name (node_ast n).
+Definition n_in (n:node) := LustreAst.n_in (node_ast n).
+Definition n_out (n:node) := LustreAst.n_out (node_ast n).
+Definition n_locals (n:node) := LustreAst.n_locals (node_ast n).
+Definition n_body (n:node) := LustreAst.n_body (node_ast n).
+
+
+Definition TBool := LustreAst.TBool.
+Definition exp := LustreAst.exp.
+Definition EConst := LustreAst.EConst.
+
+
 
 Definition node_eq (n1 n2: node) :=
   n_name n1 = n_name n2 /\
@@ -92,318 +44,8 @@ Definition node_eq (n1 n2: node) :=
   Permutation (n_locals n1) (n_locals n2) /\
   Permutation (n_body n1) (n_body n2).
 
-
-Definition var_bool := (0, TBool).
-
-Definition name_dec := String.string_dec.
-
-
-Fixpoint var_of_exp_aux (e: exp) (acc: list ident): list ident :=
-  match e with
-    | EConst _ => acc
-    | EInput _ => acc
-    | EVar (name, _) => name :: acc
-    | EUnop _ e => var_of_exp_aux e acc
-    | EBinop _ e1 e2 =>
-      var_of_exp_aux e1 (var_of_exp_aux e2 acc)
-    | EIfte e1 e2 e3 =>
-      var_of_exp_aux e1 (var_of_exp_aux e2 (var_of_exp_aux e3 acc))
-  end.
-
-Definition var_of_exp (e: exp): list ident :=
-  var_of_exp_aux e [].
-
-
-(** ** Equality of binders *)
-
-Definition type_eqb (x y: type): bool :=
-  match x, y with
-    | TVoid, TVoid => true
-    | TBool, TBool => true
-    | TInt, TInt => true
-    | _, _ => false
-  end.
-
-Lemma type_eqb_refl (t: type):
-  type_eqb t t = true.
-Proof.
-  destruct t; reflexivity.
-Qed.
-
-Lemma type_dec (x y: type): {x = y} + {x <> y}.
-Proof.
-  destruct x, y.
-  1, 5, 9: left; reflexivity.
-  all: right; inversion 1.
-Defined.
-
-Definition binder_eqb (x y: binder): bool :=
-  andb (fst x =? fst y) (type_eqb (snd x) (snd y)).
-
-Lemma binder_dec (x y: binder): {x = y} + {x <> y}.
-Proof.
-  destruct x, y.
-
-  pose proof (PeanoNat.Nat.eq_dec i i0).
-  destruct H.
-  2: {
-    right.
-    inversion 1.
-    contradiction.
-  }
-
-  destruct (type_dec t t0).
-  2: {
-    right.
-    inversion 1.
-    contradiction.
-  }
-
-  subst.
-  left.
-  reflexivity.
-Defined.
-
-Lemma binder_eqb_refl (b: binder):
-  binder_eqb b b = true.
-Proof.
-  destruct b as (i, t).
-  apply andb_true_intro.
-  split.
-  - apply PeanoNat.Nat.eqb_refl.
-  - apply type_eqb_refl.
-Qed.
-
-Lemma binder_eqb_to_eq (x y : binder): binder_eqb x y = true -> x = y.
-Proof.
-  unfold binder_eqb, andb.
-  destruct (fst x =? fst y) eqn:Heq; [| discriminate ].
-
-  rewrite PeanoNat.Nat.eqb_eq in Heq.
-  destruct x, y; simpl in Heq |- *.
-  rewrite Heq.
-
-  intros H.
-  now destruct t, t0.
-Qed.
-
-Lemma binder_eq_to_eqb (x y : binder): x = y -> binder_eqb x y = true.
-Proof.
-  unfold binder_eqb, andb.
-  destruct x, y; simpl.
-
-  inversion 1.
-
-  rewrite PeanoNat.Nat.eqb_refl.
-  now destruct t, t0.
-Qed.
-
-
-(** ** Equality of equations *)
-
-Definition unop_eqb (x y: unop): bool :=
-  match x, y with
-    | Uop_not, Uop_not => true
-    | Uop_neg, Uop_neg => true
-    | _, _ => false
-  end.
-
-Definition binop_eqb (x y: binop): bool :=
-  match x, y with
-    | Bop_and, Bop_and => true
-    | Bop_or, Bop_or => true
-    | Bop_xor, Bop_xor => true
-    | Bop_plus, Bop_plus => true
-    | Bop_minus, Bop_minus => true
-    | Bop_mult, Bop_mult => true
-    | Bop_div, Bop_div => true
-    | Bop_eq, Bop_eq => true
-    | Bop_lt, Bop_lt => true
-    | Bop_le, Bop_le => true
-    | Bop_gt, Bop_gt => true
-    | Bop_ge, Bop_ge => true
-    | _, _ => false
-  end.
-
-Definition const_eqb (c1 c2: const): bool :=
-  match c1, c2 with
-    | CVoid, CVoid => true
-    | CBool b1, CBool b2 => Bool.eqb b1 b2
-    | CInt n1, CInt n2 => PeanoNat.Nat.eqb n1 n2
-    | _, _ => false
-  end.
-
-Fixpoint exp_eqb (e1 e2: exp): bool :=
-  match e1, e2 with
-    | EConst c1, EConst c2 => const_eqb c1 c2
-    | EInput b1, EInput b2 => binder_eqb b1 b2
-    | EVar b1, EVar b2 => binder_eqb b1 b2
-    | EUnop op1 e1, EUnop op2 e2 =>
-      (unop_eqb op1 op2) && (exp_eqb e1 e2)
-    | EBinop op1 e11 e12, EBinop op2 e21 e22 =>
-      (binop_eqb op1 op2) && (exp_eqb e11 e21) && (exp_eqb e12 e22)
-    | EIfte e11 e12 e13, EIfte e21 e22 e23 =>
-      (exp_eqb e11 e21) && (exp_eqb e12 e22) && (exp_eqb e13 e23)
-    | _, _ => false
-  end.
-
-Lemma unop_eqb_refl (op: unop):
-  unop_eqb op op = true.
-Proof.
-  destruct op; reflexivity.
-Qed.
-
-Lemma unop_eqb_to_eq (op1 op2: unop):
-  unop_eqb op1 op2 = true -> op1 = op2.
-Proof.
-  intros H.
-  destruct op1, op2; (reflexivity || inversion H).
-Qed.
-
-Lemma binop_eqb_refl (op: binop):
-  binop_eqb op op = true.
-Proof.
-  destruct op; reflexivity.
-Qed.
-
-Lemma binop_eqb_to_eq (op1 op2: binop):
-  binop_eqb op1 op2 = true -> op1 = op2.
-Proof.
-  intros H.
-  destruct op1, op2; reflexivity || inversion H.
-Qed.
-
-Lemma const_eqb_refl (c: const):
-  const_eqb c c = true.
-Proof.
-  destruct c as [ | b | n ].
-  - reflexivity.
-  - apply Bool.eqb_true_iff.
-    reflexivity.
-  - apply PeanoNat.Nat.eqb_refl.
-Qed.
-
-Lemma const_eqb_to_eq (c1 c2: const):
-  const_eqb c1 c2 = true -> c1 = c2.
-Proof.
-  intros H.
-  destruct c1.
-  - destruct c2.
-    + reflexivity.
-    + inversion H.
-    + inversion H.
-  - destruct c2.
-    + inversion H.
-    + simpl in H.
-      f_equal.
-      apply Bool.eqb_true_iff.
-      assumption.
-    + inversion H.
-  - destruct c2.
-    + inversion H.
-    + inversion H.
-    + apply PeanoNat.Nat.eqb_eq in H.
-      subst.
-      reflexivity.
-Qed.
-
-Lemma exp_eqb_refl (e: exp):
-  exp_eqb e e = true.
-Proof.
-  induction e.
-  - apply const_eqb_refl.
-  - apply binder_eqb_refl.
-  - apply binder_eqb_refl.
-  - apply andb_true_intro.
-    split; [ | assumption ].
-    apply unop_eqb_refl.
-  - apply andb_true_intro.
-    split; [ | assumption ].
-    apply andb_true_intro.
-    split; [ | assumption ].
-    apply binop_eqb_refl.
-  - simpl.
-    rewrite IHe1, IHe2, IHe3.
-    reflexivity.
-Qed.
-
-Lemma exp_eqb_to_eq (e1 e2: exp):
-  exp_eqb e1 e2 = true -> e1 = e2.
-Proof.
-  intros H.
-  revert e2 H.
-  induction e1 as [ c1 | b1 | b1 | op1 e1 IH | op1 e11 IH1 e12 IH2 | e11 IH1 e12 IH2 e13 IH3 ]; intros e2 H.
-  - destruct e2; try inversion H.
-    apply const_eqb_to_eq in H1.
-    subst.
-    reflexivity.
-  - destruct e2; try inversion H.
-    apply binder_eqb_to_eq in H1.
-    subst.
-    reflexivity.
-  - destruct e2; try inversion H.
-    apply binder_eqb_to_eq in H1.
-    subst.
-    reflexivity.
-  -  destruct e2; try inversion H.
-    apply andb_prop in H1 as [ H1 H2 ].
-    apply unop_eqb_to_eq in H1.
-    apply IH in H2.
-    f_equal; assumption.
-  - destruct e2; try inversion H.
-    apply andb_prop in H1 as [ H1 H2 ].
-    apply andb_prop in H1 as [ H3 H1 ].
-    apply IH1 in H1.
-    apply IH2 in H2.
-    apply binop_eqb_to_eq in H3.
-    rewrite H1, H2, H3.
-    reflexivity.
-  - destruct e2; try inversion H.
-    apply andb_prop in H1 as [ H1 H3 ].
-    apply andb_prop in H1 as [ H1 H2 ].
-    apply IH1 in H1.
-    apply IH2 in H2.
-    apply IH3 in H3.
-    f_equal; assumption.
-Qed.
-
-Definition equation_eqb (eq1 eq2: equation): bool :=
-  (fst eq1 =? fst eq2) && (exp_eqb (snd eq1) (snd eq2)).
-
-Lemma equation_eqb_to_eq (eq1 eq2: equation):
-  equation_eqb eq1 eq2 = true -> eq1 = eq2.
-Proof.
-  intros H.
-  destruct eq1, eq2.
-  apply andb_prop in H as [ H1 H2 ].
-  apply PeanoNat.Nat.eqb_eq in H1.
-  apply exp_eqb_to_eq in H2.
-  simpl in H1, H2.
-  rewrite H1, H2.
-  reflexivity.
-Qed.
-
-Lemma equation_eqb_refl (eq: equation):
-  equation_eqb eq eq = true.
-Proof.
-  destruct eq as (i, e).
-  apply andb_true_intro.
-  split.
-  - apply PeanoNat.Nat.eqb_refl.
-  - apply exp_eqb_refl.
-Qed.
-
-Lemma equation_eq_to_eqb (eq1 eq2: equation):
-  eq1 = eq2 -> equation_eqb eq1 eq2 = true.
-Proof.
-  intros H.
-  rewrite H.
-  apply equation_eqb_refl.
-Qed.
-
-
 (** ** Semantics *)
-
+Import LustreAst.
 Inductive value :=
   | VConst : const -> value
   | VInput : binder -> value
@@ -432,7 +74,7 @@ Inductive sem_exp: history -> exp -> value -> Prop :=
       sem_exp h e1 v1 ->
       sem_exp h e2 v2 ->
       sem_exp h (EBinop op e1 e2) (VBinop op v1 v2)
-      
+
   | SeIfte (h: history) (e1 e2 e3: exp) (v1 v2 v3: value):
       sem_exp h e1 v1 ->
       sem_exp h e2 v2 ->
@@ -622,15 +264,15 @@ Proof.
     rewrite Hv1, Hv2.
     reflexivity.
   - rewrite var_of_exp_ifte_eq in H.
-    apply Forall_app in H as [ H1 H2 ]. 
+    apply Forall_app in H as [ H1 H2 ].
     apply Forall_app in H2 as [ H2 H3 ].
-    apply IH1 in H1 as [ v1 Hv1 ]. 
-    apply IH2 in H2 as [ v2 Hv2 ]. 
+    apply IH1 in H1 as [ v1 Hv1 ].
+    apply IH2 in H2 as [ v2 Hv2 ].
     apply IH3 in H3 as [ v3 Hv3 ].
     exists (VIfte v1 v2 v3).
     simpl.
     rewrite Hv1, Hv2, Hv3.
-    reflexivity. 
+    reflexivity.
 Qed.
 
 Lemma exp_evaluable_have_evaluable_vars (e: exp) (h: history) (v: value):
