theories/Translations/LustreAstToLustre.v
@@ -1,0 +1,119 @@
+From Reactive Require Import Base.
+
+From Reactive.Datatypes Require Result.
+From Reactive.Languages Require LustreAst Lustre.
+
+From Coq Require Import Sorting Permutation.
+
+Module Source := LustreAst.
+Module Target := Lustre.
+
+Definition nvars (entry: Source.node) :=
+  Source.n_in entry ++ (Source.n_out entry) :: (Source.n_locals entry).
+
+Definition n_assigned_vars (entry: Source.node) :=
+  map fst (Source.n_body entry).
+
+Open Scope string_scope.
+
+Definition check_assigned_vars_are_vars (entry: Source.node): Result.t (incl (n_assigned_vars entry) (map fst (nvars entry))).
+Proof.
+  destruct entry.
+  induction n_body.
+  - apply Result.Ok.
+    apply incl_nil_l.
+  - inversion IHn_body.
+    + destruct (ListDec.incl_dec PeanoNat.Nat.eq_dec (map fst (a::n_body)) (map fst (n_in ++ n_out :: n_locals)) ).
+      * apply Result.Ok. assumption.
+      * apply Result.Err, "A variable is never defined".
+    + apply Result.Err, H.
+Defined.
+
+
+Definition check_assigned_out (entry: Source.node): Result.t (In (fst (LustreAst.n_out entry)) (n_assigned_vars entry)).
+Proof.
+  destruct entry.
+  induction n_body.
+  - apply Result.Err, "The output variable is never assigned".
+  - destruct (ListDec.In_dec PeanoNat.Nat.eq_dec (fst n_out) (map fst (a::n_body))).
+    + simpl.
+      apply Result.Ok; assumption.
+    + apply Result.Err, "The output variable is never assigned".
+Defined.
+
+Definition n_out_is_not_an_input (entry: Source.node) :
+  Result.t (~ In (LustreAst.n_out entry) (LustreAst.n_in entry)).
+Proof.
+  destruct entry.
+  induction n_in.
+  - simpl. apply Result.Ok.
+    auto.
+  - simpl.
+    apply Result.Err, "todo".
+Defined.
+
+Scheme Equality for list.
+
+Module EquationOrder <: Orders.TotalLeBool.
+  Local Coercion is_true : bool >-> Sortclass.
+
+  Definition t := LustreAst.equation.
+
+  Definition leb (x y: LustreAst.equation): bool := Nat.leb (fst x) (fst y).
+  Infix "<=?" := leb (at level 70, no associativity).
+
+  Theorem leb_total: forall x y, x <=? y \/ y <=? x.
+  Proof.
+    intros [] [].
+    unfold leb; simpl.
+
+    revert i i0.
+    induction i; destruct i0; simpl; auto.
+  Qed.
+End EquationOrder.
+
+Module Import EquationSort := Sort EquationOrder.
+Definition list_eq_dec_equation :=
+  list_eq_dec _ LustreAst.equation_eqb LustreAst.equation_eqb_to_eq LustreAst.equation_eq_to_eqb.
+
+Definition n_inputs_equations (entry: Source.node):
+  Result.t (incl (List.map (fun b => (fst b, LustreAst.EInput b)) (LustreAst.n_in entry)) (LustreAst.n_body entry)).
+Proof.
+  destruct entry.
+  simpl.
+  induction n_body.
+  - apply Result.Err, "the body is empty".
+  - inversion IHn_body.
+    + apply Result.Ok.
+      apply incl_tl. assumption.
+    + apply Result.Err, H.
+Defined.
+
+Definition n_no_einputs_in_other (entry: Source.node):
+  Result.t (Forall (fun '(name, exp) => ~ In name (map fst (LustreAst.n_in entry)) -> LustreAst.has_einput exp = false) (LustreAst.n_body entry)).
+Proof.
+  destruct entry.
+  simpl.
+  induction n_body.
+  - apply Result.Ok.
+    apply Forall_nil.
+  - apply Result.Err, "todo".
+Defined.
+
+Import Result.notations.
+
+Definition check_node_prop (entry: Source.node): Result.t Target.node :=
+  let assigned_vars := n_assigned_vars entry in
+  do assigned_vars_are_vars <- check_assigned_vars_are_vars entry;
+  do check_assigned <- check_assigned_out entry;
+  do n_out_is_not_an_input <- n_out_is_not_an_input entry;
+  do n_inputs_equations <- n_inputs_equations entry;
+  do n_no_einputs_in_other <- n_no_einputs_in_other entry;
+  Result.Ok {|
+      Target.node_ast := entry;
+      Target.n_assigned_vars_are_vars := assigned_vars_are_vars;
+      Target.n_assigned_out := check_assigned;
+      Target.n_out_is_not_an_input := n_out_is_not_an_input;
+      Target.n_inputs_equations := n_inputs_equations;
+      Target.n_no_einputs_in_other := n_no_einputs_in_other
+    |}.
